wrote most of load function, changed perennial to opam package

src/proof/hashtriemap/model.v
@@ -82,268 +82,268 @@ Section model.
       (belongs_to_path p)
       (full_domain).
 
-  (* Definition path_ok (p : path) : Prop := *)
-  (*   length p ≤ 16 ∧ Forall (λ n, n ∈ nibble_list) p. *)
+  (* (* Definition path_ok (p : path) : Prop := *) *)
+  (* (*   length p ≤ 16 ∧ Forall (λ n, n ∈ nibble_list) p. *) *)
 
-  (* Definition P (p : path) k : Prop := *)
-  (*   k ≫ (sh p) = pref p. *)
+  (* (* Definition P (p : path) k : Prop := *) *)
+  (* (*   k ≫ (sh p) = pref p. *) *)
 
-  Lemma path_to_prefix_snoc (p : path) (n : nibble) :
-    path_to_prefix (p ++ [n]) =
-    ((path_to_prefix p) ≪ 4) + n.
-  Proof.
-    unfold path_to_prefix.
-    (* use foldl_app; stdpp has foldl_app, otherwise prove it *)
-    rewrite foldl_app.
-    simpl.
-    reflexivity.
-  Qed.
+  (* Lemma path_to_prefix_snoc (p : path) (n : nibble) : *)
+  (*   path_to_prefix (p ++ [n]) = *)
+  (*   ((path_to_prefix p) ≪ 4) + n. *)
+  (* Proof. *)
+  (*   unfold path_to_prefix. *)
+  (*   (* use foldl_app; stdpp has foldl_app, otherwise prove it *) *)
+  (*   rewrite foldl_app. *)
+  (*   simpl. *)
+  (*   reflexivity. *)
+  (* Qed. *)
 
-  (* TODO: replace all the 4's with hashtriemap.nChildrenLog2, 16 with hashtriemap.nChildren *)
+  (* (* TODO: replace all the 4's with hashtriemap.nChildrenLog2, 16 with hashtriemap.nChildren *) *)
 
-  Lemma sh_snoc (p : path) (n : nibble) :
-    sh (p ++ [n]) = sh p - 4.
-  Proof.
-    unfold sh.
-    rewrite app_length /=.
-    lia.
-  Qed.
+  (* Lemma sh_snoc (p : path) (n : nibble) : *)
+  (*   sh (p ++ [n]) = sh p - 4. *)
+  (* Proof. *)
+  (*   unfold sh. *)
+  (*   rewrite app_length /=. *)
+  (*   lia. *)
+  (* Qed. *)
 
-  Lemma sh_nonneg (p : path) :
-    (Z.of_nat (length p) < 64 `div` 4)%Z ->
-    0 ≤ sh p.
-  Proof.
-    unfold sh.
-    word.
-  Qed.
+  (* Lemma sh_nonneg (p : path) : *)
+  (*   (Z.of_nat (length p) < 64 `div` 4)%Z -> *)
+  (*   0 ≤ sh p. *)
+  (* Proof. *)
+  (*   unfold sh. *)
+  (*   word. *)
+  (* Qed. *)
 
-  Lemma shiftr_eq_iff_interval (p : path) (u : Z) :
-    0 ≤ sh p ->
-    0 ≤ u ->
-    (u ≫ (sh p) = path_to_prefix p) ↔ (lo p ≤ u < hi p).
-  Proof.
-    intros Hsh_nonneg Hu_nonneg.
-    repeat unfold lo, hi in *.
-    set (pp := path_to_prefix p) in *.
-    set (s := sh p) in *.
-    repeat rewrite Z.shiftr_div_pow2; try word.
-    repeat rewrite Z.shiftl_mul_pow2; try word.
-    set (b := 2 ^ s) in *.
-    have Hbne : b > 0.
-    { unfold b. word. }
+  (* Lemma shiftr_eq_iff_interval (p : path) (u : Z) : *)
+  (*   0 ≤ sh p -> *)
+  (*   0 ≤ u -> *)
+  (*   (u ≫ (sh p) = path_to_prefix p) ↔ (lo p ≤ u < hi p). *)
+  (* Proof. *)
+  (*   intros Hsh_nonneg Hu_nonneg. *)
+  (*   repeat unfold lo, hi in *. *)
+  (*   set (pp := path_to_prefix p) in *. *)
+  (*   set (s := sh p) in *. *)
+  (*   repeat rewrite Z.shiftr_div_pow2; try word. *)
+  (*   repeat rewrite Z.shiftl_mul_pow2; try word. *)
+  (*   set (b := 2 ^ s) in *. *)
+  (*   have Hbne : b > 0. *)
+  (*   { unfold b. word. } *)
 
-    split.
-    - intro H.
-      rewrite (Z.div_mod u b).
-      2: { word. }
-      rewrite H.
-      split.
-      + word.
-      + have Hmod : 0 <= u mod b < b by apply Z.mod_pos_bound; lia.
-        lia.
-    - intros [Hlo Hhi].
-      have H : (pp = u `div` b ↔ u `div` b = pp) by word.
-      rewrite -H.
-      apply (Z.div_unique u b pp (u - pp*b)).
-      + lia.
-      + have : 0 <= u - pp*b < b by lia.
-        word.
-  Qed.
+  (*   split. *)
+  (*   - intro H. *)
+  (*     rewrite (Z.div_mod u b). *)
+  (*     2: { word. } *)
+  (*     rewrite H. *)
+  (*     split. *)
+  (*     + word. *)
+  (*     + have Hmod : 0 <= u mod b < b by apply Z.mod_pos_bound; lia. *)
+  (*       lia. *)
+  (*   - intros [Hlo Hhi]. *)
+  (*     have H : (pp = u `div` b ↔ u `div` b = pp) by word. *)
+  (*     rewrite -H. *)
+  (*     apply (Z.div_unique u b pp (u - pp*b)). *)
+  (*     + lia. *)
+  (*     + have : 0 <= u - pp*b < b by lia. *)
+  (*       word. *)
+  (* Qed. *)
 
-  Lemma interval_split (p : path) (n : Z) :
-    4 ≤ sh p ->
-    lo (p ++ [n]) = lo p + n * (2 ^ (sh p - 4)).
-  Proof.
-    (* expand lo, use path_to_prefix_snoc + sh_snoc + shiftl algebra *)
-    intros Hsh_nonneg.
-    unfold lo.
-    rewrite path_to_prefix_snoc.
-    rewrite sh_snoc.
-    simpl.
-    repeat rewrite Z.shiftl_mul_pow2; try word.
-    rewrite Z.mul_add_distr_r.
-    have Hpow : 2 ^ 4 * 2 ^ (sh p - 4) = 2 ^ (sh p).
-    {
-      rewrite -Z.pow_add_r; try word.
-      simpl.
-      have H : 4 + (sh p - 4) = sh p by word.
-      rewrite H.
-      reflexivity.
-    }
-    replace (path_to_prefix p * 2 ^ 4 * 2 ^ (sh p - 4) + n * 2 ^ (sh p - 4)) with (path_to_prefix p * 2 ^ sh p + n * 2 ^ (sh p - 4)) by word.
-    done.
-  Qed.
+  (* Lemma interval_split (p : path) (n : Z) : *)
+  (*   4 ≤ sh p -> *)
+  (*   lo (p ++ [n]) = lo p + n * (2 ^ (sh p - 4)). *)
+  (* Proof. *)
+  (*   (* expand lo, use path_to_prefix_snoc + sh_snoc + shiftl algebra *) *)
+  (*   intros Hsh_nonneg. *)
+  (*   unfold lo. *)
+  (*   rewrite path_to_prefix_snoc. *)
+  (*   rewrite sh_snoc. *)
+  (*   simpl. *)
+  (*   repeat rewrite Z.shiftl_mul_pow2; try word. *)
+  (*   rewrite Z.mul_add_distr_r. *)
+  (*   have Hpow : 2 ^ 4 * 2 ^ (sh p - 4) = 2 ^ (sh p). *)
+  (*   { *)
+  (*     rewrite -Z.pow_add_r; try word. *)
+  (*     simpl. *)
+  (*     have H : 4 + (sh p - 4) = sh p by word. *)
+  (*     rewrite H. *)
+  (*     reflexivity. *)
+  (*   } *)
+  (*   replace (path_to_prefix p * 2 ^ 4 * 2 ^ (sh p - 4) + n * 2 ^ (sh p - 4)) with (path_to_prefix p * 2 ^ sh p + n * 2 ^ (sh p - 4)) by word. *)
+  (*   done. *)
+  (* Qed. *)
 
-  Lemma interval_consecutive (p : path) (n : Z) :
-    4 ≤ sh p ->
-    hi (p ++ [n]) = lo (p ++ [n+1]).
-  Proof.
-    intros Hsh_nonneg.
-    repeat unfold hi, lo in *.
-    repeat rewrite path_to_prefix_snoc.
-    repeat rewrite sh_snoc.
-    have H : path_to_prefix p ≪ 4 + n + 1 = path_to_prefix p ≪ 4 + (n + 1) by lia.
-    rewrite H.
-    reflexivity.
-  Qed.
+  (* Lemma interval_consecutive (p : path) (n : Z) : *)
+  (*   4 ≤ sh p -> *)
+  (*   hi (p ++ [n]) = lo (p ++ [n+1]). *)
+  (* Proof. *)
+  (*   intros Hsh_nonneg. *)
+  (*   repeat unfold hi, lo in *. *)
+  (*   repeat rewrite path_to_prefix_snoc. *)
+  (*   repeat rewrite sh_snoc. *)
+  (*   have H : path_to_prefix p ≪ 4 + n + 1 = path_to_prefix p ≪ 4 + (n + 1) by lia. *)
+  (*   rewrite H. *)
+  (*   reflexivity. *)
+  (* Qed. *)
 
-  Lemma full_domain_elem (k : w64) :
-    uint.Z k ∈ full_domain.
-  Proof.
-    unfold full_domain.
-    apply elem_of_seqZ; word.
-  Qed.
+  (* Lemma full_domain_elem (k : w64) : *)
+  (*   uint.Z k ∈ full_domain. *)
+  (* Proof. *)
+  (*   unfold full_domain. *)
+  (*   apply elem_of_seqZ; word. *)
+  (* Qed. *)
 
-  Lemma path_to_domain_elem (p : path) (k : Z) :
-    k ∈ full_domain →
-    k ∈ path_to_domain p ↔ k ≫ sh p = path_to_prefix p.
-  Proof.
-    intro Hk.
-    unfold path_to_domain.
-    rewrite list_elem_of_filter.
-    split; intro H.
-    - destruct H as [Hk' Hpred].
-      exact Hk'.
-    - split; done.
-  Qed.
+  (* Lemma path_to_domain_elem (p : path) (k : Z) : *)
+  (*   k ∈ full_domain → *)
+  (*   k ∈ path_to_domain p ↔ k ≫ sh p = path_to_prefix p. *)
+  (* Proof. *)
+  (*   intro Hk. *)
+  (*   unfold path_to_domain. *)
+  (*   rewrite list_elem_of_filter. *)
+  (*   split; intro H. *)
+  (*   - destruct H as [Hk' Hpred]. *)
+  (*     exact Hk'. *)
+  (*   - split; done. *)
+  (* Qed. *)
 
-  Lemma nibble_list_range (n : Z) :
-    n ∈ nibble_list ↔ 0 ≤ n < 16.
-  Proof.
-    apply elem_of_seqZ.
-  Qed.
+  (* Lemma nibble_list_range (n : Z) : *)
+  (*   n ∈ nibble_list ↔ 0 ≤ n < 16. *)
+  (* Proof. *)
+  (*   apply elem_of_seqZ. *)
+  (* Qed. *)
 
-  Lemma next_nibble_exists (p : path) (k : Z) :
-    0 ≤ k →
-    length p < 16 ->
-    belongs_to_path p k ->
-    ∃ n, 0 ≤ n < 16 ∧ belongs_to_path (p ++ [n]) k.
-  Proof.
-    intros Hk Hlen Hbelong.
-    unfold belongs_to_path in *.
-    unfold lo, hi in *.
-    set (s := sh p) in *.
-    set (pp := path_to_prefix p) in *.
-    have Hinterval : pp ≪ s ≤ k < (pp + 1) ≪ s.
-    {
-      apply shiftr_eq_iff_interval; [|word|word].
-      unfold sh.
-      word.
-    }
-    set (n := Z.land (k ≫ (s - 4)) (Z.ones 4)).
-    exists n.
-    split.
-    - (* show 0 ≤ n < 16 *)
-      unfold n.
-      set (x := k ≫ (s - 4)).
-      have Hland : Z.land x 15 = x mod 2^4.
-      { change 15 with (Z.ones 4) in *. rewrite Z.land_ones; auto. word. }
-      rewrite Hland. apply Z.mod_pos_bound.
-      word.
-    - (* show belongs_to_path (p ++ [n]) k *)
-      unfold belongs_to_path.
-      have Hs : 4 ≤ sh p.
-      {
-        unfold sh.
-        word.
-      }
-      replace (sh (p ++ [n])) with (s - 4) by (rewrite sh_snoc; word).
-      rewrite path_to_prefix_snoc.
-      set (x := k ≫ (s-4)).
-      assert (Hxmod : x mod 16 = n).
-      {
-        subst x n. change 16 with (2^4).
-        rewrite Z.land_ones; try word.
-      }
-      assert (Hxdiv : x / 16 = pp).
-      {
-        subst x.
-        rewrite Z.shiftr_div_pow2; [|word].
-        rewrite Z.shiftr_div_pow2 in Hbelong; [|word].
-        rewrite Z.pow_sub_r; try word.
-        rewrite -Hbelong.
-        replace (2^4) with 16 by word.
-        set (x := 2^s).
-        have Hxge16 : (16 ≤ x).
-        {
-          unfold x, s.
-          change (16 ≤ 2 ^ sh p) with (2 ^ 4 ≤ 2 ^ (sh p)).
-          apply Z.pow_le_mono_r; lia.
-        }
-        rewrite Z.div_div; [|word|word].
-        have Hx : x mod 16 = 0.
-        {
-          unfold x.
-          have Ht : s mod 4 = 0 by (unfold s, sh; word).
-          have Hdiv : Z.divide 4 s.
-          { apply Z.mod_divide; lia. }
-          destruct Hdiv as [y Hy].
-          replace (y * 4) with (4 * y) in Hy by word.
-          rewrite Hy.
-          rewrite Z.pow_mul_r; [|word|word].
-          replace (2^4) with 16 by word.
-          have Hypos : 1 ≤ y by lia.
-          have Hdiv : Z.divide 16 (16 ^ y).
-          {
-            exists (16 ^ (y - 1)).
-            replace y with (y - 1 + 1) by lia.
-            rewrite Z.pow_succ_r; [|word].
-            simpl.
-            replace (y - 1 + 1 - 1) with (y - 1) by word.
-            word.
-          }
-          rewrite Z.mod_divide; [|word].
-          exact Hdiv.
-        }
-        replace (x / 16 * 16) with (x) by word.
-        reflexivity.
-      }
-      have Hx : x = pp * 16 + n.
-      {
-        rewrite (Z.div_mod x 16); word.
-      }
-      change 16 with (2^4) in Hx.
-      rewrite -Z.shiftl_mul_pow2 in Hx; try word.
-      exact Hx.
-  Qed.
+  (* Lemma next_nibble_exists (p : path) (k : Z) : *)
+  (*   0 ≤ k → *)
+  (*   length p < 16 -> *)
+  (*   belongs_to_path p k -> *)
+  (*   ∃ n, 0 ≤ n < 16 ∧ belongs_to_path (p ++ [n]) k. *)
+  (* Proof. *)
+  (*   intros Hk Hlen Hbelong. *)
+  (*   unfold belongs_to_path in *. *)
+  (*   unfold lo, hi in *. *)
+  (*   set (s := sh p) in *. *)
+  (*   set (pp := path_to_prefix p) in *. *)
+  (*   have Hinterval : pp ≪ s ≤ k < (pp + 1) ≪ s. *)
+  (*   { *)
+  (*     apply shiftr_eq_iff_interval; [|word|word]. *)
+  (*     unfold sh. *)
+  (*     word. *)
+  (*   } *)
+  (*   set (n := Z.land (k ≫ (s - 4)) (Z.ones 4)). *)
+  (*   exists n. *)
+  (*   split. *)
+  (*   - (* show 0 ≤ n < 16 *) *)
+  (*     unfold n. *)
+  (*     set (x := k ≫ (s - 4)). *)
+  (*     have Hland : Z.land x 15 = x mod 2^4. *)
+  (*     { change 15 with (Z.ones 4) in *. rewrite Z.land_ones; auto. word. } *)
+  (*     rewrite Hland. apply Z.mod_pos_bound. *)
+  (*     word. *)
+  (*   - (* show belongs_to_path (p ++ [n]) k *) *)
+  (*     unfold belongs_to_path. *)
+  (*     have Hs : 4 ≤ sh p. *)
+  (*     { *)
+  (*       unfold sh. *)
+  (*       word. *)
+  (*     } *)
+  (*     replace (sh (p ++ [n])) with (s - 4) by (rewrite sh_snoc; word). *)
+  (*     rewrite path_to_prefix_snoc. *)
+  (*     set (x := k ≫ (s-4)). *)
+  (*     assert (Hxmod : x mod 16 = n). *)
+  (*     { *)
+  (*       subst x n. change 16 with (2^4). *)
+  (*       rewrite Z.land_ones; try word. *)
+  (*     } *)
+  (*     assert (Hxdiv : x / 16 = pp). *)
+  (*     { *)
+  (*       subst x. *)
+  (*       rewrite Z.shiftr_div_pow2; [|word]. *)
+  (*       rewrite Z.shiftr_div_pow2 in Hbelong; [|word]. *)
+  (*       rewrite Z.pow_sub_r; try word. *)
+  (*       rewrite -Hbelong. *)
+  (*       replace (2^4) with 16 by word. *)
+  (*       set (x := 2^s). *)
+  (*       have Hxge16 : (16 ≤ x). *)
+  (*       { *)
+  (*         unfold x, s. *)
+  (*         change (16 ≤ 2 ^ sh p) with (2 ^ 4 ≤ 2 ^ (sh p)). *)
+  (*         apply Z.pow_le_mono_r; lia. *)
+  (*       } *)
+  (*       rewrite Z.div_div; [|word|word]. *)
+  (*       have Hx : x mod 16 = 0. *)
+  (*       { *)
+  (*         unfold x. *)
+  (*         have Ht : s mod 4 = 0 by (unfold s, sh; word). *)
+  (*         have Hdiv : Z.divide 4 s. *)
+  (*         { apply Z.mod_divide; lia. } *)
+  (*         destruct Hdiv as [y Hy]. *)
+  (*         replace (y * 4) with (4 * y) in Hy by word. *)
+  (*         rewrite Hy. *)
+  (*         rewrite Z.pow_mul_r; [|word|word]. *)
+  (*         replace (2^4) with 16 by word. *)
+  (*         have Hypos : 1 ≤ y by lia. *)
+  (*         have Hdiv : Z.divide 16 (16 ^ y). *)
+  (*         { *)
+  (*           exists (16 ^ (y - 1)). *)
+  (*           replace y with (y - 1 + 1) by lia. *)
+  (*           rewrite Z.pow_succ_r; [|word]. *)
+  (*           simpl. *)
+  (*           replace (y - 1 + 1 - 1) with (y - 1) by word. *)
+  (*           word. *)
+  (*         } *)
+  (*         rewrite Z.mod_divide; [|word]. *)
+  (*         exact Hdiv. *)
+  (*       } *)
+  (*       replace (x / 16 * 16) with (x) by word. *)
+  (*       reflexivity. *)
+  (*     } *)
+  (*     have Hx : x = pp * 16 + n. *)
+  (*     { *)
+  (*       rewrite (Z.div_mod x 16); word. *)
+  (*     } *)
+  (*     change 16 with (2^4) in Hx. *)
+  (*     rewrite -Z.shiftl_mul_pow2 in Hx; try word. *)
+  (*     exact Hx. *)
+  (* Qed. *)
 
-  Lemma next_nibble_unique (p : path) (k : Z) n1 n2 :
-    belongs_to_path (p ++ [n1]) k ->
-    belongs_to_path (p ++ [n2]) k ->
-    n1 = n2.
-  Proof.
-    intros H1 H2.
-    unfold belongs_to_path in *.
-    have Hlen : sh (p ++ [n1]) = sh (p ++ [n2]) by
-                                   rewrite !sh_snoc; lia.
-    rewrite Hlen in H1.
-    (* now both equal the same LHS *)
-    have Hpref : path_to_prefix (p ++ [n1]) = path_to_prefix (p ++ [n2]) by
-                                                etrans; [symmetry; exact H1| exact H2].
-    rewrite !path_to_prefix_snoc in Hpref.
-    word.
-  Qed.
+  (* Lemma next_nibble_unique (p : path) (k : Z) n1 n2 : *)
+  (*   belongs_to_path (p ++ [n1]) k -> *)
+  (*   belongs_to_path (p ++ [n2]) k -> *)
+  (*   n1 = n2. *)
+  (* Proof. *)
+  (*   intros H1 H2. *)
+  (*   unfold belongs_to_path in *. *)
+  (*   have Hlen : sh (p ++ [n1]) = sh (p ++ [n2]) by *)
+  (*                                  rewrite !sh_snoc; lia. *)
+  (*   rewrite Hlen in H1. *)
+  (*   (* now both equal the same LHS *) *)
+  (*   have Hpref : path_to_prefix (p ++ [n1]) = path_to_prefix (p ++ [n2]) by *)
+  (*                                               etrans; [symmetry; exact H1| exact H2]. *)
+  (*   rewrite !path_to_prefix_snoc in Hpref. *)
+  (*   word. *)
+  (* Qed. *)
 
-  Lemma path_to_domain_split (p : path) :
-    length p < 16 ->            (* length p < (sizeof hashT) / nChildrenLog2 *)
-    path_to_domain p =
-    concat (map (λ n, path_to_domain (p ++ [n])) nibble_list).
-  Proof.
-    intro Hlen.
-    apply list_eq. intros.
-    apply option_eq; intro k.
-    split; intro H.
-    - (* → *)
-      apply list_elem_of_lookup_2 in H.
-      rewrite list_elem_of_filter in H.
-      destruct H as [Hbelong Hfull].
-      (* Hfull: k ∈ full_domain *)
-      rewrite elem_of_seqZ in Hfull.
-      have Hk_nonneg : 0 ≤ k := proj1 Hfull.
-      destruct (next_nibble_exists p k) as [x [Hnrange Hbelongn]];
-        try done.
-      set (l := concat (map (λ n : nibble, path_to_domain (p ++ [n])) nibble_list)).
-  Admitted.
+  (* Lemma path_to_domain_split (p : path) : *)
+  (*   length p < 16 ->            (* length p < (sizeof hashT) / nChildrenLog2 *) *)
+  (*   path_to_domain p = *)
+  (*   concat (map (λ n, path_to_domain (p ++ [n])) nibble_list). *)
+  (* Proof. *)
+  (*   intro Hlen. *)
+  (*   apply list_eq. intros. *)
+  (*   apply option_eq; intro k. *)
+  (*   split; intro H. *)
+  (*   - (* → *) *)
+  (*     apply list_elem_of_lookup_2 in H. *)
+  (*     rewrite list_elem_of_filter in H. *)
+  (*     destruct H as [Hbelong Hfull]. *)
+  (*     (* Hfull: k ∈ full_domain *) *)
+  (*     rewrite elem_of_seqZ in Hfull. *)
+  (*     have Hk_nonneg : 0 ≤ k := proj1 Hfull. *)
+  (*     destruct (next_nibble_exists p k) as [x [Hnrange Hbelongn]]; *)
+  (*       try done. *)
+  (*     set (l := concat (map (λ n : nibble, path_to_domain (p ++ [n])) nibble_list)). *)
+  (* Admitted. *)
 
   Definition hash_map : Type := gmap Z (gmap K V). (* TODO: should be gmap hashT (gmap K V), its just Z for now to make the above helper lemmas easier *)
 
@@ -367,20 +367,16 @@ Section model.
   Definition singleton_map_fn (h: Z) (m: gmap K V) : Z → gmap K V :=
     λ h', if decide (h' = h) then m else ∅.
 
-  Definition null_child
-    (γ: ghost_names) (q: Qp) (path: path) : iProp Σ :=
-    own_path γ.(map_name) q path empty_map_fn.
-
   Fixpoint entry_chain_struct (q: Qp) (kvs: list (K * V)) (ent: loc) : iProp Σ :=
     match kvs with
     | [] => ⌜ent = null⌝%I
     | kv :: rest =>
         (
           ⌜ent ≠ null⌝ ∗
-          ∃ (overflow_field overflow_loc: loc),
-            ent ↦s[hashtriemap.entry :: "key"]{DfracOwn q} (fst kv) ∗
-            ent ↦s[hashtriemap.entry :: "value"]{DfracOwn q} (snd kv) ∗
-            ent ↦s[hashtriemap.entry :: "overflow"]{DfracOwn q} overflow_field ∗
+          ∃ overflow_field (overflow_loc: loc),
+            ent ↦s[hashtriemap.entry :: "key"]□ (fst kv) ∗
+            ent ↦s[hashtriemap.entry :: "value"]□ (snd kv) ∗
+            (* ent ↦s[hashtriemap.entry :: "overflow"]{DfracOwn q} overflow_field ∗ *)
             own_Value overflow_field (DfracOwn q)
               (interface.mk (ptrT.id hashtriemap.entry.id) #overflow_loc) ∗
             entry_chain_struct q rest overflow_loc
@@ -388,72 +384,86 @@ Section model.
     end.
 
   Definition entry
-    (γ: ghost_names) (q: Qp) (e: loc) (path: path) : iProp Σ :=
-    ∃ (kvs: list (K * V)) (h: Z),
+    (kvs: list (K * V)) h (q: Qp) (e: loc) (path: path) : iProp Σ :=
       entry_chain_struct q kvs e ∗
       ⌜kvs ≠ []⌝ ∗
       ⌜NoDup (fst <$> kvs)⌝ ∗
-      ⌜∀ kv, kv ∈ kvs → uint.Z (hash_key kv.1) = h⌝ ∗
-             ⌜belongs_to_path path h⌝ ∗
-             own_path γ.(map_name) q path (singleton_map_fn h (list_to_map kvs)).
+      (⌜∀ kv, kv ∈ kvs → uint.Z (hash_key kv.1) = h⌝) ∗
+      ⌜belongs_to_path path h⌝.
 
   Definition childrenP
-    (γ: ghost_names) (q: Qp)
-    (child_indirect: loc → path → iProp Σ)
+    (child_indirect: loc -d> path -d> iProp Σ)
+    (γ: ghost_names) (q: Qp) (children_slice: slice.t)
+    (children_vals: list atomic.Value.t)
     (ind: loc) (path: path) : iProp Σ :=
-    ∃ (children_locs: list loc),
-      ind ↦s[hashtriemap.indirect :: "children"]{DfracOwn q} children_locs ∗
-      ⌜length children_locs = 16%nat⌝ ∗
-      (
-        [∗ list] i ↦ cloc ∈ children_locs,
-          let child_path := path ++ [Z.of_nat i] in
-          ∃ (nptr: loc),
-            own_Value cloc (DfracOwn q)
-              (interface.mk (ptrT.id hashtriemap.node.id) #nptr) ∗
-            (
-              (  ⌜nptr = null⌝ ∗ null_child γ q child_path)
-              ∨ (⌜nptr ≠ null⌝ ∗
-                 ∃ (is_entry: bool),
-                   nptr ↦s[hashtriemap.node :: "isEntry"]{DfracOwn q} is_entry ∗
-                   if is_entry then
-                     entry γ q (struct.field_ref_f hashtriemap.node "ent" nptr) child_path
-                   else
-                     child_indirect (struct.field_ref_f hashtriemap.node "ind" nptr) child_path)
-            )
-      ).
+    "Hchildren" :: [∗ list] i ↦ val ∈ children_vals,
+      let child_path := path ++ [Z.of_nat i] in
+      ∃ (nodeptr: loc),
+        "Hown_child" :: own_Value (slice.elem_ref_f children_slice atomic.Value i) (DfracOwn q)
+          (interface.mk (ptrT.id hashtriemap.node.id) #nodeptr) ∗
+        (
+          if (decide (nodeptr = null)) then
+            own_path γ.(map_name) q child_path empty_map_fn
+          else
+            ∃ (is_entry: bool),
+              nodeptr ↦s[hashtriemap.node :: "isEntry"]□ is_entry ∗
+              if is_entry then
+                ∃ kvs h,
+                  own_path γ.(map_name) q path (singleton_map_fn h (list_to_map kvs)) ∗
+                  entry kvs h q (struct.field_ref_f hashtriemap.node "ent" nodeptr) child_path
+              else
+                ▷ child_indirect (struct.field_ref_f hashtriemap.node "ind" nodeptr) child_path).
 
-  Definition max_depth : nat := 16.
+  (* split 50/50 between an invariant and the mutex to allow for lock-free reads *)
+  (* we always have read permission on any indirect, but only can write if we acquire the lock *)
+  (* the only things ever modified are atomic values (atomic pointers), everything else is □ ownership *)
+  Definition indirect_F
+    (γ: ghost_names)
+    (indirect: loc -d> (list Z) -d> iProp Σ)
+    : loc -d> (list Z) -d> iProp Σ :=
+    λ ind path,
+      (∃ (children_vals: list atomic.Value.t) children_slice,
+          "#Hown_children" :: ind ↦s[hashtriemap.indirect :: "children"]□ children_slice ∗
+          "#Hchildren_slice" :: children_slice ↦*□ children_vals ∗
+          "%Hchildren_len" :: ⌜length children_vals = 16%nat⌝ ∗
+          "#Hind_inv" :: inv (indN) ((childrenP indirect γ (1/2)%Qp children_slice children_vals ind path)) ∗
+          "#Hind_mutex" :: is_Mutex (struct.field_ref_f hashtriemap.indirect "mu" ind)
+            (childrenP indirect γ (1/2)%Qp children_slice children_vals ind path))%I.
 
-  Definition depth_remaining_of_path (p: path) : nat :=
-    Z.to_nat (sh p / 4) + 1.
-
-  Fixpoint indirect
-    (γ: ghost_names) (depth_remaining: nat) (ind: loc) (path: path) : iProp Σ :=
-    match depth_remaining with
-    | O => False%I              (* something went wrong *)
-    | S d =>
-        inv (indN)
-          (childrenP γ (1/2)%Qp (λ l p, indirect γ d l p) ind path) ∗
-        is_Mutex (struct.field_ref_f hashtriemap.indirect "mu" ind)
-          (childrenP γ (1/2)%Qp (λ l p, indirect γ d l p) ind path)
-    end.
-
-  Lemma indirect_unfold γ depth ind path :
-    indirect γ (S depth) ind path ⊣⊢
-    inv (indN)
-      (childrenP γ (1/2)%Qp (λ l p, indirect γ depth l p) ind path) ∗
-    is_Mutex (struct.field_ref_f hashtriemap.indirect "mu" ind)
-      (childrenP γ (1/2)%Qp (λ l p, indirect γ depth l p) ind path).
+  (* Prove contractiveness *)
+  Global Instance indirect_F_contractive γ : Contractive (indirect_F γ).
   Proof.
-    reflexivity.
+    rewrite /indirect_F.
+    intros n f g Hfg ind path.
+    f_equiv.
+    f_equiv.
+    f_equiv.
+    f_equiv.
+    have H : ((childrenP f γ (1 / 2) a0 a ind path) ≡{n}≡ (childrenP g γ (1 / 2) a0 a ind path)).
+    { solve_contractive. }
+    repeat f_equiv; exact H.
+  Qed.
+
+  Definition indirect (γ: ghost_names) (ind: loc) (path: path) : iProp Σ :=
+    fixpoint (indirect_F γ) ind path.
+
+  Lemma indirect_unfold γ ind path :
+    indirect γ ind path ⊣⊢
+    indirect_F γ (indirect γ) ind path.
+  Proof. apply (fixpoint_unfold (indirect_F γ)). Qed.
+
+  #[global] Instance indirect_persistent γ ind path : Persistent (indirect γ ind path).
+  Proof.
+    rewrite indirect_unfold /indirect_F.
+    apply _.
   Qed.
 
   Definition ht_inv (ht: loc) (γ: ghost_names) : iProp Σ :=
-    ∃ (i: loc) (hm: hash_map),
-      map_ctx γ.(map_name) 1 hm ∗
-      own_Value (struct.field_ref_f hashtriemap.HashTrieMap "root" ht) DfracDiscarded
-        (interface.mk (ptrT.id hashtriemap.indirect.id) #i) ∗
-      indirect γ (S max_depth) i [].
+    ∃ (rooti: loc) (hm: hash_map),
+      "Hauth_map" :: map_ctx γ.(map_name) 1 hm ∗
+      "Hown_root" :: own_Value (struct.field_ref_f hashtriemap.HashTrieMap "root" ht) DfracDiscarded
+        (interface.mk (ptrT.id hashtriemap.indirect.id) #rooti) ∗
+      "#Hroot_indirect" :: indirect γ rooti [].
 
   (* Public predicate exposed to clients. *)
   (* HOCAP style *)
@@ -508,7 +518,8 @@ Section model.
   Definition hashtriemap_init
     `{!ghost_varG Σ bool}
     (ht: loc) (γ: ghost_names) (* P *) : iProp Σ :=
-    init_status ht γ (* P *) ∗ init_mu ht γ (* ∗ P ∅ *).
+    "#Hinit" :: init_status ht γ (* P *) ∗
+    "#Hinit_mu" :: init_mu ht γ (* ∗ P ∅ *).
 
   Lemma hashtriemap_pre_auth_init
     `{!mapG Σ w64 w64, !ghost_varG Σ (gmap w64 w64), !ghost_varG Σ bool} :
